* ensuring that magics in the code are all in ghost contexts, with one exception * linked lists append with a while loop, forall* and @==>; lots of annotations ..., but it works

pulse/src/ocaml/plugin/Pulse_RuntimeUtils.ml
@@ -167,3 +167,5 @@ let get_attributes (s:S.sigelt) (ps:_) =
 
 let must_erase_for_extraction (g:FStar_Reflection_Types.env) (ty:FStar_Syntax_Syntax.term) =
   FStar_TypeChecker_Util.must_erase_for_extraction g ty
+
+let magic_s s = failwith ("Cannot execute magic: " ^ s)
