pulse/src/ocaml/plugin/generated/Pulse_Soundness_Sub.ml
@@ -1,14 +1,1 @@
 open Prims
-let (app_typing :
-  FStar_Reflection_Types.env ->
-    FStar_Reflection_Types.term ->
-      FStar_Reflection_Types.term ->
-        FStar_Reflection_Types.term ->
-          FStar_Reflection_Types.term ->
-            (unit, unit, unit) FStar_Reflection_Typing.tot_typing ->
-              (unit, unit, unit) FStar_Reflection_Typing.tot_typing ->
-                (unit, unit, unit) FStar_Reflection_Typing.tot_typing)
-  =
-  fun g ->
-    fun ty1 ->
-      fun ty2 -> fun f -> fun tm -> fun df -> fun dt -> Prims.magic ()
