pulse/lib/steel/pulse/Pulse.Typing.Metatheory.Base.fst
@@ -24,8 +24,8 @@ let admit_comp_typing (g:env) (c:comp_st)
 let st_typing_correctness_ctot (#g:env) (#t:st_term) (#c:comp{C_Tot? c}) 
                                (_:st_typing g t c)
 : (u:Ghost.erased universe & universe_of g (comp_res c) u)
-= let u : Ghost.erased universe = RU.magic_s "st_typing_correctness_ctot.u" in
-  let ty : universe_of g (comp_res c) u = RU.magic_s "st_typing_correctness_ctot.universe_of" in
+= let u : Ghost.erased universe = RU.magic () in
+  let ty : universe_of g (comp_res c) u = RU.magic() in
   (| u, ty |)    
 
 let st_typing_correctness (#g:env) (#t:st_term) (#c:comp_st) 
@@ -71,7 +71,7 @@ let non_informative_t_weakening (g g':env) (g1:env{ pairwise_disjoint g g1 g' })
   (d:non_informative_t (push_env g g') u t)
   : non_informative_t (push_env (push_env g g1) g') u t =
   let (| w, _ |) = d in
-  (| w, magic () |)
+  (| w, RU.magic #(tot_typing _ _ _) () |)
 
 let non_informative_c_weakening (g g':env) (g1:env{ pairwise_disjoint g g1 g' })
   (c:comp_st)
@@ -90,19 +90,19 @@ let bind_comp_weakening (g:env) (g':env { disjoint g g' })
     assume (None? (lookup (push_env g g1) x));
     let y = fresh (push_env (push_env g g1) g') in
     assume (~ (y `Set.mem` (freevars (comp_post c2))));
-    Bind_comp _ x c1 c2 (magic ()) y (magic ())
+    Bind_comp _ x c1 c2 (RU.magic ()) y (RU.magic ())
 
   | Bind_comp_ghost_l _ x c1 c2 n_d _ _ _ ->
     assume (None? (lookup (push_env g g1) x));
     let y = fresh (push_env (push_env g g1) g') in
     assume (~ (y `Set.mem` (freevars (comp_post c2))));
-    Bind_comp_ghost_l _ x c1 c2 (non_informative_c_weakening g g' g1 _ n_d) (magic ()) y (magic ())
+    Bind_comp_ghost_l _ x c1 c2 (non_informative_c_weakening g g' g1 _ n_d) (RU.magic ()) y (RU.magic ())
 
   | Bind_comp_ghost_r _ x c1 c2 n_d _ _ _ ->
     assume (None? (lookup (push_env g g1) x));
     let y = fresh (push_env (push_env g g1) g') in
     assume (~ (y `Set.mem` (freevars (comp_post c2))));
-    Bind_comp_ghost_r _ x c1 c2 (non_informative_c_weakening g g' g1 _ n_d) (magic ()) y (magic ())
+    Bind_comp_ghost_r _ x c1 c2 (non_informative_c_weakening g g' g1 _ n_d) (RU.magic ()) y (RU.magic ())
   
 let lift_comp_weakening (g:env) (g':env { disjoint g g'})
   (#c1 #c2:comp) (d:lift_comp (push_env g g') c1 c2)
@@ -125,7 +125,7 @@ let st_equiv_weakening (g:env) (g':env { disjoint g g' })
     assume (~ (x `Set.mem` dom g'));
     assume (~ (x `Set.mem` dom g1));
     // TODO: the proof for RT.Equiv is not correct here
-    ST_VPropEquiv _ c1 c2 x (magic ()) (magic ()) (magic ()) (FStar.Reflection.Typing.Rel_refl _ _ _) (magic ()) (magic ())
+    ST_VPropEquiv _ c1 c2 x (RU.magic ()) (RU.magic ()) (RU.magic ()) (FStar.Reflection.Typing.Rel_refl _ _ _) (RU.magic ()) (RU.magic ())
 #pop-options
 
 // TODO: add precondition that g1 extends g'
@@ -164,19 +164,19 @@ let st_comp_typing_weakening (g:env) (g':env { disjoint g g' })
   | STC _ st x _ _ _ ->
     assume (~ (x `Set.mem` dom g'));
     assume (~ (x `Set.mem` dom g1));
-    STC _ st x (magic ()) (magic ()) (magic ())
+    STC _ st x (RU.magic ()) (RU.magic ()) (RU.magic ())
 
 let comp_typing_weakening (g:env) (g':env { disjoint g g' })
   (#c:comp) (#u:universe) (d:comp_typing (push_env g g') c u)
   (g1:env { pairwise_disjoint g g1 g' })
   : comp_typing (push_env (push_env g g1) g') c u =
   match d with
-  | CT_Tot _ t u _ -> CT_Tot _ t u (magic ())
+  | CT_Tot _ t u _ -> CT_Tot _ t u (RU.magic ())
   | CT_ST _ _ d -> CT_ST _ _ (st_comp_typing_weakening g g' d g1)
   | CT_STAtomic _ inames _ _ d ->
-    CT_STAtomic _ inames _ (magic ()) (st_comp_typing_weakening g g' d g1)
+    CT_STAtomic _ inames _ (RU.magic ()) (st_comp_typing_weakening g g' d g1)
   | CT_STGhost _ inames _ _ d ->
-    CT_STGhost _ inames _ (magic ()) (st_comp_typing_weakening g g' d g1)
+    CT_STGhost _ inames _ (RU.magic ()) (st_comp_typing_weakening g g' d g1)
 
 #push-options "--split_queries no --z3rlimit_factor 8 --fuel 1 --ifuel 1"
 let rec st_typing_weakening g g' t c d g1
@@ -184,18 +184,20 @@ let rec st_typing_weakening g g' t c d g1
         (decreases d) =
   
   match d with
-  | T_Abs _ _ _ _ _ _ _ _ _ ->
+  | T_Abs g x q b u body c b_typing body_typing ->
     // T_Abs is used only at the top, should not come up
-    magic ()
-
+    assume false;
+    let x = fresh (push_env (push_env g g1) g') in
+    T_Abs g x q b u body c (RU.magic #(tot_typing _ _ _) ()) 
+                          (st_typing_weakening g g' body c body_typing g1)
   | T_STApp _ head ty q res arg _ _ ->
-    T_STApp _ head ty q res arg (magic ()) (magic ())
+    T_STApp _ head ty q res arg (RU.magic #(tot_typing _ _ _) ()) (RU.magic #(tot_typing _ _ _) ())
 
   | T_STGhostApp _ head ty q res arg _ _ _ _ ->
     // candidate for renaming
     let x = fresh (push_env (push_env g g1) g') in
     assume (~ (x `Set.mem` freevars_comp res));
-    T_STGhostApp _ head ty q res arg x (magic ()) (magic ()) (magic ())
+    T_STGhostApp _ head ty q res arg x (RU.magic ()) (RU.magic ()) (RU.magic ())
 
   | T_Return _ c use_eq u t e post x_old _ _ _ ->
     let x = fresh (push_env (push_env g g1) g') in
@@ -203,7 +205,7 @@ let rec st_typing_weakening g g' t c d g1
     // x is only used to open and then close
     assume (comp_return c use_eq u t e post x_old ==
             comp_return c use_eq u t e post x);
-    T_Return _ c use_eq u t e post x (magic ()) (magic ()) (magic ())
+    T_Return _ c use_eq u t e post x (RU.magic ()) (RU.magic ()) (RU.magic ())
 
   | T_Lift _ e c1 c2 d_c1 d_lift ->
     T_Lift _ e c1 c2 (st_typing_weakening g g' e c1 d_c1 g1)
@@ -241,7 +243,7 @@ let rec st_typing_weakening g g' t c d g1
                   (open_st_term_nv e2 (b.binder_ppname, x))
                   c2 = d_e2 in
     let d_bc = bind_comp_weakening g g' d_bc g1 in
-    T_Bind _ e1 e2 c1 c2 b x c d_e1 (magic ()) d_e2 d_bc
+    T_Bind _ e1 e2 c1 c2 b x c d_e1 (RU.magic ()) d_e2 d_bc
 
   | T_BindFn _ e1 e2 c1 c2 b x d_e1 u _ d_e2 c2_typing  ->
     let d_e1 : st_typing (push_env (push_env g g1) g') e1 c1 =
@@ -274,7 +276,8 @@ let rec st_typing_weakening g g' t c d g1
       : st_typing (push_binding (push_env (push_env g g1) g') x ppname_default (comp_res c1))
                   (open_st_term_nv e2 (b.binder_ppname, x))
                   c2 = d_e2 in
-    T_BindFn _ e1 e2 c1 c2 b x d_e1 u (magic()) d_e2 (magic())
+    let c2_typing = comp_typing_weakening g g' c2_typing g1 in
+    T_BindFn _ e1 e2 c1 c2 b x d_e1 u (RU.magic #(tot_typing _ _ _) ()) d_e2 c2_typing
 
   | T_TotBind _ e1 e2 t1 c2 b x _ d_e2 ->
     assume (~ (x `Set.mem` dom g'));
@@ -300,7 +303,7 @@ let rec st_typing_weakening g g' t c d g1
                   (open_st_term_nv e2 (v_as_nv x))
                   c2 = d_e2 in
     
-    T_TotBind _ e1 e2 t1 c2 b x (magic ()) d_e2
+    T_TotBind _ e1 e2 t1 c2 b x (RU.magic ()) d_e2
 
   | T_GhostBind _ e1 e2 t1 c2 b x _ d_e2 _ ->
     assume (~ (x `Set.mem` dom g'));
@@ -326,7 +329,7 @@ let rec st_typing_weakening g g' t c d g1
                   (open_st_term_nv e2 (v_as_nv x))
                   c2 = d_e2 in
     
-    T_GhostBind _ e1 e2 t1 c2 b x (magic ()) d_e2 (magic ())
+    T_GhostBind _ e1 e2 t1 c2 b x (RU.magic ()) d_e2 (RU.magic ())
 
 
   | T_If _ b e1 e2 c uc hyp _ d_e1 d_e2 _ ->
@@ -365,7 +368,7 @@ let rec st_typing_weakening g g' t c d g1
       : st_typing (push_binding (push_env (push_env g g1) g') hyp ppname_default (mk_eq2 u0 tm_bool b tm_false))
                   e2 c = d_e2 in
 
-    T_If _ b e1 e2 c uc hyp (magic ()) d_e1 d_e2 (magic ())
+    T_If _ b e1 e2 c uc hyp (RU.magic ()) d_e1 d_e2 (RU.magic ())
   
   | T_Match _ sc_u sc_ty sc d_sc_ty d_sc c brs d_brs d_pats_complete ->
     admit();
@@ -378,7 +381,7 @@ let rec st_typing_weakening g g' t c d g1
             d_pats_complete
 
   | T_Frame _ e c frame _ d_e ->
-    T_Frame _ e c frame (magic ()) (st_typing_weakening g g' e c d_e g1)
+    T_Frame _ e c frame (RU.magic ()) (st_typing_weakening g g' e c d_e g1)
 
   | T_Equiv _ e c c' d_e d_eq ->
     T_Equiv _ e c c' (st_typing_weakening g g' e c d_e g1) (st_equiv_weakening g g' d_eq g1)
@@ -386,18 +389,18 @@ let rec st_typing_weakening g g' t c d g1
   | T_Sub _ e c c' d_e d_sub ->
     T_Sub _ e c c' (st_typing_weakening g g' e c d_e g1) (st_sub_weakening g g' d_sub g1)
 
-  | T_IntroPure _ p _ token -> T_IntroPure _ p (magic ()) (prop_validity_token_weakening token _)
+  | T_IntroPure _ p _ token -> T_IntroPure _ p (RU.magic ()) (prop_validity_token_weakening token _)
 
   | T_ElimExists _ u t p x _ _ ->
     assume (~ (x `Set.mem` dom g'));
     assume (~ (x `Set.mem` dom g1));
-    T_ElimExists _ u t p x (magic ()) (magic ())
+    T_ElimExists _ u t p x (RU.magic ()) (RU.magic ())
 
   | T_IntroExists _ u b p e _ _ _ ->
-    T_IntroExists _ u b p e (magic ()) (magic ()) (magic ())
+    T_IntroExists _ u b p e (RU.magic ()) (RU.magic ()) (RU.magic ())
 
   | T_While _ inv cond body _ cond_typing body_typing ->
-    T_While _ inv cond body (magic ())
+    T_While _ inv cond body (RU.magic ())
       (st_typing_weakening g g' cond (comp_while_cond ppname_default inv) cond_typing g1)
       (st_typing_weakening g g' body (comp_while_body ppname_default inv) body_typing g1)
 
@@ -434,7 +437,7 @@ let rec st_typing_weakening g g' t c d g1
       : st_typing (push_binding (push_env (push_env g g1) g') x ppname_default (mk_ref init_t))
                   (open_st_term_nv body (v_as_nv x))
                   (comp_withlocal_body x init_t init c) = d_body in
-    T_WithLocal _ ppname init body init_t c x (magic ()) (magic ())
+    T_WithLocal _ ppname init body init_t c x (RU.magic ()) (RU.magic ())
       (comp_typing_weakening g g' d_c g1)
       d_body
 
@@ -462,11 +465,11 @@ let rec st_typing_weakening g g' t c d g1
       : st_typing (push_binding (push_env (push_env g g1) g') x ppname_default (mk_array init_t))
                   (open_st_term_nv body (v_as_nv x))
                   (comp_withlocal_array_body x init_t init len c) = d_body in
-    T_WithLocalArray _ ppname init len body init_t c x (magic ()) (magic ()) (magic ())
+    T_WithLocalArray _ ppname init len body init_t c x (RU.magic ()) (RU.magic ()) (RU.magic ())
       (comp_typing_weakening g g' d_c g1)
       d_body
 
-  | T_Rewrite _ p q _ _ -> T_Rewrite _ p q (magic ()) (magic ())
+  | T_Rewrite _ p q _ _ -> T_Rewrite _ p q (RU.magic ()) (RU.magic ())
 
   | T_Admit _ s c d_s -> T_Admit _ s c (st_comp_typing_weakening g g' d_s g1)
 
@@ -489,7 +492,7 @@ let non_informative_t_subst (g:env) (x:var) (t:typ) (g':env { pairwise_disjoint 
   let ss = nt x e in
 
   let (| w, _ |) = d in
-  (| subst_term w ss, magic () |)
+  (| subst_term w ss, RU.magic #(tot_typing _ _ _) () |)
 
 let non_informative_c_subst (g:env) (x:var) (t:typ) (g':env { pairwise_disjoint g (singleton_env (fstar_env g) x t) g' })
   (#e:term)
@@ -539,25 +542,25 @@ let bind_comp_subst
   | Bind_comp _ y c1 c2 _ z _ ->
     Bind_comp _ y (subst_comp c1 ss)
                   (subst_comp c2 ss)
-                  (magic ())
+                  (RU.magic ())
                   z
-                  (magic ())
+                  (RU.magic ())
   
   | Bind_comp_ghost_l _ y c1 c2 d_non_informative _ z _ ->
     Bind_comp_ghost_l _ y (subst_comp c1 ss)
                           (subst_comp c2 ss)
                           (non_informative_c_subst g x t g' e_typing _ d_non_informative)
-                          (magic ())
+                          (RU.magic ())
                           z
-                          (magic ())
+                          (RU.magic ())
 
   | Bind_comp_ghost_r _ y c1 c2 d_non_informative _ z _ ->
     Bind_comp_ghost_r _ y (subst_comp c1 ss)
                           (subst_comp c2 ss)
                           (non_informative_c_subst g x t g' e_typing _ d_non_informative)
-                          (magic ())
+                          (RU.magic ())
                           z
-                          (magic ())
+                          (RU.magic ())
 
 let st_equiv_subst (g:env) (x:var) (t:typ) (g':env { pairwise_disjoint g (singleton_env (fstar_env g) x t) g' })
   (#e:term)
@@ -571,12 +574,12 @@ let st_equiv_subst (g:env) (x:var) (t:typ) (g':env { pairwise_disjoint g (single
     ST_VPropEquiv _ (subst_comp c1 (nt x e))
                     (subst_comp c2 (nt x e))
                     y
-                    (magic ())
-                    (magic ())
-                    (magic ())
+                    (RU.magic ())
+                    (RU.magic ())
+                    (RU.magic ())
                     (RT.Rel_refl _ _ _)  // TODO: incorrect proof
-                    (magic ())
-                    (magic ())
+                    (RU.magic ())
+                    (RU.magic ())
 
 let st_comp_typing_subst (g:env) (x:var) (t:typ) (g':env { pairwise_disjoint g (singleton_env (fstar_env g) x t) g' })
   (#e:term)
@@ -588,9 +591,9 @@ let st_comp_typing_subst (g:env) (x:var) (t:typ) (g':env { pairwise_disjoint g (
   | STC _ s y _ _ _ ->
     STC _ (subst_st_comp s (nt x e))
          y
-         (magic ())
-         (magic ())
-         (magic ())
+         (RU.magic ())
+         (RU.magic ())
+         (RU.magic ())
 
 let comp_typing_subst (g:env) (x:var) (t:typ) (g':env { pairwise_disjoint g (singleton_env (fstar_env g) x t) g' })
   (#e:term)
@@ -600,13 +603,13 @@ let comp_typing_subst (g:env) (x:var) (t:typ) (g':env { pairwise_disjoint g (sin
                 (subst_comp c (nt x e)) u =
   match d with
   | CT_Tot _ t u _ ->
-    CT_Tot _ (subst_term t (nt x e)) u (magic ())
+    CT_Tot _ (subst_term t (nt x e)) u (RU.magic ())
   | CT_ST _ s d_s ->
     CT_ST _ (subst_st_comp s (nt x e)) (st_comp_typing_subst g x t g' e_typing d_s)
   | CT_STAtomic _ inames s _ d_s ->
-    CT_STAtomic _ inames (subst_st_comp s (nt x e)) (magic ()) (st_comp_typing_subst g x t g' e_typing d_s)
+    CT_STAtomic _ inames (subst_st_comp s (nt x e)) (RU.magic ()) (st_comp_typing_subst g x t g' e_typing d_s)
   | CT_STGhost _ inames s _ d_s ->
-    CT_STGhost _ inames (subst_st_comp s (nt x e)) (magic ()) (st_comp_typing_subst g x t g' e_typing d_s)
+    CT_STGhost _ inames (subst_st_comp s (nt x e)) (RU.magic ()) (st_comp_typing_subst g x t g' e_typing d_s)
   
 
 let coerce_eq (#a #b:Type) (x:a) (_:squash (a == b)) : y:b { y == x } = x
@@ -620,7 +623,8 @@ let rec st_typing_subst g x t g' #e #eff e_typing #e1 #c1 e1_typing _
   let ss = nt x e in
 
   match e1_typing with
-  | T_Abs _ _ _ _ _ _ _ _ _ -> magic ()
+  | T_Abs _ _ _ _ _ _ _ _ _ ->
+    Pervasives.coerce_eq (RU.magic ()) e1_typing
 
   | T_STApp _ head ty q res arg _ _ ->
     T_STApp _ (subst_term head ss)
@@ -628,19 +632,19 @@ let rec st_typing_subst g x t g' #e #eff e_typing #e1 #c1 e1_typing _
               q
               (subst_comp res ss)
               (subst_term arg ss)
-              (magic ())
-              (magic ())
+              (RU.magic ())
+              (RU.magic ())
 
-  | T_STGhostApp _ head ty q res arg x _ _ _ ->
+ | T_STGhostApp _ head ty q res arg x _ _ _ ->
     T_STGhostApp _ (subst_term head ss)
               (subst_term ty ss)
               q
               (subst_comp res ss)
               (subst_term arg ss)
               x
-              (magic ())
-              (magic ())
-              (magic ())
+              (RU.magic ())
+              (RU.magic ())
+              (RU.magic ())
 
   | T_Return _ c use_eq u t e post x _ _ _ ->
     T_Return _ c use_eq u
@@ -648,15 +652,15 @@ let rec st_typing_subst g x t g' #e #eff e_typing #e1 #c1 e1_typing _
       (subst_term e ss)
       (subst_term post ss)
       x
-      (magic ())
-      (magic ())
-      (magic ())
+      (RU.magic ())
+      (RU.magic ())
+      (RU.magic ())
 
   | T_Lift _ e c1 c2 d_e d_lift ->
     T_Lift _ (subst_st_term e ss)
              (subst_comp c1 ss)
              (subst_comp c2 ss)
-             (st_typing_subst g x t g' e_typing d_e (magic ()))
+             (st_typing_subst g x t g' e_typing d_e (RU.magic ()))
              (lift_comp_subst g x t g' e_typing d_lift)
 
   | T_Bind _ e1 e2 c1 c2 b y c d_e1 _ d_e2 d_bc ->
@@ -667,9 +671,9 @@ let rec st_typing_subst g x t g' #e #eff e_typing #e1 #c1 e1_typing _
              (subst_binder b ss)
              y
              (subst_comp c ss)
-             (st_typing_subst g x t g' e_typing d_e1 (magic ()))
-             (magic ())
-             (coerce_eq (st_typing_subst g x t (push_binding g' y ppname_default (comp_res c1)) e_typing d_e2 (magic ())) ())
+             (st_typing_subst g x t g' e_typing d_e1 (RU.magic ()))
+             (RU.magic ())
+             (coerce_eq (st_typing_subst g x t (push_binding g' y ppname_default (comp_res c1)) e_typing d_e2 (RU.magic ())) ())
              (bind_comp_subst g x t g' e_typing d_bc)
 
   | T_BindFn _ e1 e2 c1 c2 b y d_e1 u _ d_e2 d_c2 ->
@@ -679,12 +683,11 @@ let rec st_typing_subst g x t g' #e #eff e_typing #e1 #c1 e1_typing _
                (subst_comp c2 ss)
                (subst_binder b ss)
                y
-               (st_typing_subst g x t g' e_typing d_e1 (magic ()))
+               (st_typing_subst g x t g' e_typing d_e1 (RU.magic ()))
                u
-               (magic ())
-               (coerce_eq (st_typing_subst g x t (push_binding g' y ppname_default (comp_res c1)) e_typing d_e2 (magic ())) ())
+               (RU.magic ())
+               (coerce_eq (st_typing_subst g x t (push_binding g' y ppname_default (comp_res c1)) e_typing d_e2 (RU.magic ())) ())
                (comp_typing_subst g x t (push_binding g' y ppname_default (comp_res c1)) e_typing d_c2)
-
   | T_TotBind _ e1 e2 t1 c2 b y _ d_e2 ->
     T_TotBind _ (subst_term e1 ss)
                 (subst_st_term e2 ss)
@@ -692,8 +695,8 @@ let rec st_typing_subst g x t g' #e #eff e_typing #e1 #c1 e1_typing _
                 (subst_comp c2 ss)
                 b
                 y
-                (magic ())
-                (coerce_eq (st_typing_subst g x t (push_binding g' y ppname_default t1) e_typing d_e2 (magic ())) ())
+                (RU.magic ())
+                (coerce_eq (st_typing_subst g x t (push_binding g' y ppname_default t1) e_typing d_e2 (RU.magic ())) ())
 
   | T_GhostBind _ e1 e2 t1 c2 b y _ d_e2 _ ->
     T_GhostBind _ (subst_term e1 ss)
@@ -702,9 +705,9 @@ let rec st_typing_subst g x t g' #e #eff e_typing #e1 #c1 e1_typing _
                 (subst_comp c2 ss)
                 b
                 y
-                (magic ())
-                (coerce_eq (st_typing_subst g x t (push_binding g' y ppname_default t1) e_typing d_e2 (magic ())) ())
-                (magic ())
+                (RU.magic ())
+                (coerce_eq (st_typing_subst g x t (push_binding g' y ppname_default t1) e_typing d_e2 (RU.magic ())) ())
+                (RU.magic ())
 
   | T_If _ b e1 e2 c uc hyp _ d_e1 d_e2 _ ->
     T_If _ (subst_term b ss)
@@ -713,50 +716,51 @@ let rec st_typing_subst g x t g' #e #eff e_typing #e1 #c1 e1_typing _
            (subst_comp c ss)
            uc
            hyp
-           (magic ())
-           (coerce_eq (st_typing_subst g x t (push_binding g' hyp ppname_default (mk_eq2 u0 tm_bool b tm_true)) e_typing d_e1 (magic ())) ())
-           (coerce_eq (st_typing_subst g x t (push_binding g' hyp ppname_default (mk_eq2 u0 tm_bool b tm_false)) e_typing d_e2 (magic ())) ())
-           (magic ())
+           (RU.magic ())
+           (coerce_eq (st_typing_subst g x t (push_binding g' hyp ppname_default (mk_eq2 u0 tm_bool b tm_true)) e_typing d_e1 (RU.magic ())) ())
+           (coerce_eq (st_typing_subst g x t (push_binding g' hyp ppname_default (mk_eq2 u0 tm_bool b tm_false)) e_typing d_e2 (RU.magic ())) ())
+           (RU.magic ())
 
-  | T_Match _ _ _ _ _ _ _ _ _ _ -> magic ()
+  | T_Match _ sc_u sc_ty sc _ty_typing _sc_typing c brs brs_typing pats_complete ->
+    Pervasives.coerce_eq (RU.magic ()) e1_typing
 
   | T_Frame _ e c frame _ d_e ->
     T_Frame _ (subst_st_term e ss)
               (subst_comp c ss)
               (subst_term frame ss)
-              (magic ())
-              (st_typing_subst g x t g' e_typing d_e (magic ()))
+              (RU.magic ())
+              (st_typing_subst g x t g' e_typing d_e (RU.magic ()))
 
   | T_Equiv _ e c c' d_e d_eq ->
     T_Equiv _ (subst_st_term e ss)
               (subst_comp c ss)
               (subst_comp c' ss)
-              (st_typing_subst g x t g' e_typing d_e (magic ()))
+              (st_typing_subst g x t g' e_typing d_e (RU.magic ()))
               (st_equiv_subst g x t g' e_typing d_eq)
 
   | T_IntroPure _ p _ _ ->
     T_IntroPure _ (subst_term p ss)
-                  (magic ())
-                  (magic ())
+                  (RU.magic ())
+                  (RU.magic ())
 
   | T_ElimExists _ u t p y _ _ ->
-    T_ElimExists _ u (subst_term t ss) (subst_term p ss) y (magic ()) (magic ())
+    T_ElimExists _ u (subst_term t ss) (subst_term p ss) y (RU.magic ()) (RU.magic ())
 
   | T_IntroExists _ u b p e _ _ _ ->
     T_IntroExists _ u (subst_binder b ss)
                       (subst_term p ss)
                       (subst_term e ss)
-                      (magic ())
-                      (magic ())
-                      (magic ())
+                      (RU.magic ())
+                      (RU.magic ())
+                      (RU.magic ())
 
   | T_While _ inv cond body _ cond_typing body_typing ->
     T_While _ (subst_term inv ss)
               (subst_st_term cond ss)
               (subst_st_term body ss)
-              (magic ())
-              (st_typing_subst g x t g' e_typing cond_typing (magic ()))
-              (st_typing_subst g x t g' e_typing body_typing (magic ()))
+              (RU.magic ())
+              (st_typing_subst g x t g' e_typing cond_typing (RU.magic ()))
+              (st_typing_subst g x t g' e_typing body_typing (RU.magic ()))
 
   | T_Par _ eL cL eR cR y d_cL d_cR d_eL d_eR ->
     T_Par _ (subst_st_term eL ss)
@@ -766,8 +770,8 @@ let rec st_typing_subst g x t g' #e #eff e_typing #e1 #c1 e1_typing _
             y
             (comp_typing_subst g x t g' e_typing d_cL)
             (comp_typing_subst g x t g' e_typing d_cR)
-            (st_typing_subst g x t g' e_typing d_eL (magic ()))
-            (st_typing_subst g x t g' e_typing d_eR (magic ()))
+            (st_typing_subst g x t g' e_typing d_eL (RU.magic ()))
+            (st_typing_subst g x t g' e_typing d_eR (RU.magic ()))
 
   | T_WithLocal _ ppname init body init_t c y _ _ d_c d_body ->
     T_WithLocal _ ppname
@@ -776,10 +780,10 @@ let rec st_typing_subst g x t g' #e #eff e_typing #e1 #c1 e1_typing _
                   (subst_term init_t ss)
                   (subst_comp c ss)
                   y
-                  (magic ())
-                  (magic ())
+                  (RU.magic ())
+                  (RU.magic ())
                   (comp_typing_subst g x t g' e_typing d_c)
-                  (coerce_eq (st_typing_subst g x t (push_binding g' y ppname_default (mk_ref init_t)) e_typing d_body (magic ())) ())
+                  (coerce_eq (st_typing_subst g x t (push_binding g' y ppname_default (mk_ref init_t)) e_typing d_body (RU.magic ())) ())
 
   | T_WithLocalArray _ ppname init len body init_t c y _ _ _ d_c d_body ->
     T_WithLocalArray _ ppname
@@ -789,17 +793,17 @@ let rec st_typing_subst g x t g' #e #eff e_typing #e1 #c1 e1_typing _
                        (subst_term init_t ss)
                        (subst_comp c ss)
                        y
-                       (magic ())
-                       (magic ())
-                       (magic ())
+                       (RU.magic ())
+                       (RU.magic ())
+                       (RU.magic ())
                        (comp_typing_subst g x t g' e_typing d_c)
-                       (coerce_eq (st_typing_subst g x t (push_binding g' y ppname_default (mk_ref init_t)) e_typing d_body (magic ())) ())
+                       (coerce_eq (st_typing_subst g x t (push_binding g' y ppname_default (mk_ref init_t)) e_typing d_body (RU.magic ())) ())
 
   | T_Rewrite _ p q _ _ ->
     T_Rewrite _ (subst_term p ss)
                 (subst_term q ss)
-                (magic ())
-                (magic ())
+                (RU.magic ())
+                (RU.magic ())
 
   | T_Admit _ s c d_s ->
     T_Admit _ (subst_st_comp s ss) c (st_comp_typing_subst g x t g' e_typing d_s)
